aarch64 infoflow: prove refinement
Signed-off-by: Ryan Barry <ryan.barry@proofcraft.systems>

proof/infoflow/refine/AARCH64/ArchADT_IF_Refine_C.thy
@@ -12,25 +12,6 @@ context kernel_m begin
 
 named_theorems ADT_IF_Refine_assms
 
-lemma handleInterrupt_ccorres[ADT_IF_Refine_assms]:
-  "ccorres (K dc \<currency> dc) (liftxf errstate id (K ()) ret__unsigned_long_')
-           (invs')
-           (UNIV)
-           []
-           (handleEvent Interrupt)
-           (handleInterruptEntry_C_body_if)"
-  apply (rule ccorres_guard_imp2)
-   apply (simp add: handleEvent_def minus_one_norm handleInterruptEntry_C_body_if_def)
-   apply (rule ccorres_add_return2)
-   apply (ctac (no_vcg) add: checkInterrupt_ccorres)
-    apply (rule_tac R="\<lambda>_. rv = Inr ()" in ccorres_return[where R'=UNIV])
-    apply (rule conseqPre, vcg)
-    apply (clarsimp simp: return_def)
-   apply (simp add: liftE_def)
-   apply wpsimp
-  apply clarsimp
-  done
-
 lemma handleInvocation_ccorres'[ADT_IF_Refine_assms]:
   "ccorres (K dc \<currency> dc) (liftxf errstate id (K ()) ret__unsigned_long_')
        (invs' and arch_extras and ct_active' and sch_act_simple)
@@ -182,6 +163,8 @@ lemma check_active_irq_corres_C[ADT_IF_Refine_assms]:
           apply (rule ccorres_rel_imp, rule ccorres_guard_imp)
              apply (rule getActiveIRQ_ccorres)
             apply simp+
+          apply (clarsimp split: option.splits)
+         apply simp+
        apply (rule no_fail_dmo')
        apply (rule no_fail_getActiveIRQ)
       apply (rule corres_trivial, clarsimp split: if_split option.splits)
@@ -224,10 +207,144 @@ lemma obs_cpspace_user_data_relation[ADT_IF_Refine_assms]:
   apply simp
   done
 
+
+definition handleHypervisorFault_C_body_if :: "64 word \<Rightarrow> (globals myvars, int, strictc_errortype) com"
+  where
+  "handleHypervisorFault_C_body_if hyp_fault_type ==
+      IF hyp_fault_type = 0x2000000 THEN
+        \<acute>ret__unsigned_long :== CALL getESR();;
+        \<acute>current_fault :== CALL seL4_Fault_UserException_new(\<acute>ret__unsigned_long,scast (0 :: 32 signed word));;
+        CALL handleFault(\<acute>ksCurThread)
+      ELSE
+        \<acute>current_fault :== CALL seL4_Fault_VCPUFault_new(hyp_fault_type);;
+        CALL handleFault(\<acute>ksCurThread)
+      FI;; \<acute>ret__unsigned_long :== scast EXCEPTION_NONE"
+
+definition hyp_fault_type_from_H :: "hyp_fault_type \<Rightarrow> machine_word" where
+  "hyp_fault_type_from_H fault \<equiv>
+    case fault of hyp_fault_type.ARMVCPUFault f \<Rightarrow> ucast f"
+
+lemma ucast_helper:
+  "\<lbrakk> UCAST('a::len \<rightarrow> 'b::len) a = b; LENGTH('a) \<le> LENGTH('b) \<rbrakk>
+     \<Longrightarrow> a = UCAST('b::len \<rightarrow> 'a::len) b"
+  by fastforce
+
+
+lemma handleHypervisorFault_C_body_ccorres[ADT_IF_Refine_assms]:
+  "ccorres (K dc \<currency> dc) (liftxf errstate id (K ()) ret__unsigned_long_')
+           (invs' and arch_extras and ct_running' and (\<lambda>s. ksSchedulerAction s = ResumeCurrentThread))
+           (UNIV) []
+           (liftE (do thread <- getCurThread;
+                      handleHypervisorFault thread flt
+                   od))
+           (handleHypervisorFault_C_body_if (hyp_fault_type_from_H flt))"
+  apply (rule ccorres_guard_imp)
+   apply (simp add: liftE_def bind_assoc handleHypervisorFault_C_body_if_def)
+   apply (rule ccorres_pre_getCurThread)
+   apply (rule ccorres_split_nothrow_novcg)
+
+
+       apply (simp only: handleHypervisorFault_def handleHypervisorFault_C_body_if_def hyp_fault_type_from_H_def)
+       apply wpc
+       apply (simp only: hyp_fault_type.simps)
+
+       apply (rule_tac P="ARMVCPUFault x = ARMVCPUFault 0x2000000" in ccorres_cases)
+        apply clarsimp
+        apply (rule ccorres_cond_univ)
+        apply (rule ccorres_rhs_assoc)+
+        apply (ctac (no_vcg) add: getESR_ccorres)
+         apply (rule ccorres_symb_exec_r)
+         apply (rule_tac P="\<lambda>s. ksCurThread s = thread" in ccorres_cross_over_guard)
+
+           apply (rule_tac xf'=xfdc in ccorres_call)
+              apply (ctac (no_vcg) add: handleFault_ccorres)
+             apply simp
+            apply simp
+           apply simp
+          apply vcg
+         apply (clarsimp, rule conseqPre, vcg)
+         apply clarsimp
+        apply wp
+
+apply clarsimp
+       apply (prop_tac "x \<noteq> 0x2000000")
+        apply clarsimp
+       apply clarsimp
+       apply (prop_tac "UCAST(32 \<rightarrow> 64) x \<noteq> 0x2000000")
+        apply (erule swap)
+        apply clarsimp
+        apply (drule ucast_helper)
+         apply clarsimp
+        apply clarsimp
+       apply clarsimp
+
+       apply (rule ccorres_cond_empty)
+       apply (rule ccorres_symb_exec_r)
+         apply (rule_tac P="\<lambda>s. ksCurThread s = thread" in ccorres_cross_over_guard)
+         apply (rule_tac xf'=xfdc in ccorres_call)
+            apply (ctac (no_vcg) add: handleFault_ccorres)
+           apply simp
+          apply simp
+         apply simp
+          apply vcg
+       apply (rule conseqPre, vcg)
+         apply clarsimp
+      apply ceqv
+
+      apply clarsimp
+      apply (rule_tac P=\<top> and P'=UNIV in ccorres_from_vcg)
+      apply (rule allI, rule conseqPre, vcg)
+      apply (clarsimp simp: return_def)
+
+      apply wp
+     apply (simp add: guard_is_UNIV_def)
+   apply clarsimp
+   apply (auto simp: ct_in_state'_def isReply_def is_cap_fault_def
+                     cfault_rel_def seL4_Fault_UnknownSyscall_lift seL4_Fault_UserException_lift
+                     seL4_Fault_VCPUFault_lift
+               elim: pred_tcb'_weakenE st_tcb_ex_cap''
+               dest: st_tcb_at_idle_thread' rf_sr_ksCurThread split: if_splits)[1]
+  apply (rule ucast_and_mask_drop)
+  apply clarsimp
+  done
+
+declare handleSpuriousIRQ_ccorres[ADT_IF_Refine_assms]
+declare hvmf_invs_lift[ADT_IF_Refine_assms]
+
+lemma checkInterrupt_ccorres'[ADT_IF_Refine_assms]:
+  "ccorres dc xfdc (\<lambda>s. invs' s \<and> (\<not>inKernel \<longrightarrow> sch_act_not (ksCurThread s) s)) UNIV []
+           (maybeHandleInterrupt inKernel) (Call checkInterrupt_'proc)"
+  unfolding maybeHandleInterrupt_def
+  apply cinit'
+  apply (rule ccorres_guard_imp)
+    apply (simp add: liftE_def bind_assoc)
+    apply (ctac (no_vcg) add: getActiveIRQ_ccorres)
+         apply (rule_tac P="\<lambda>_. rv \<noteq> None" and R=\<top> in ccorres_cond_both)
+           apply (auto split: option.splits)[1]
+          apply (rule_tac P="rv \<noteq> None" in ccorres_gen_asm)
+          apply clarsimp
+          apply wpfix
+          apply (rule ccorres_call[where xf'=xfdc, OF handleInterrupt_ccorres]; simp)
+         apply (rule_tac P="rv = None" in ccorres_gen_asm)
+         apply clarsimp
+         apply wpfix
+         apply (ctac (no_vcg) add: handleSpuriousIRQ_ccorres)
+      apply wp
+     apply (simp add: guard_is_UNIV_def)
+    apply (rule_tac Q'="\<lambda>rv s. invs' s \<and> (\<forall>irq. rv = Some irq \<longrightarrow> irq \<in> non_kernel_IRQs \<longrightarrow>
+                                                sch_act_not (ksCurThread s) s)"
+                    in hoare_post_imp)
+     apply (solves clarsimp)
+    apply (wpsimp wp: dmo_getActiveIRQ_inKernel_sch_act_not)
+    apply assumption
+   apply assumption
+  apply (clarsimp simp: invs'_def valid_state'_def)
+  done
+
 end
 
 
-sublocale kernel_m \<subseteq> ADT_IF_Refine_1?: ADT_IF_Refine_1 _ _ _ doUserOp_C_if
+sublocale kernel_m \<subseteq> ADT_IF_Refine_1?: ADT_IF_Refine_1 _ _ _ doUserOp_C_if handleHypervisorFault_C_body_if hyp_fault_type_from_H
 proof goal_cases
   interpret Arch .
   case 1 show ?case
